Term/WithArity/AContext.v
@@ -8,7 +8,7 @@ See the COPYRIGHTS and LICENSE files.
 one-hole contexts
 *)
 
-(* $Id: AContext.v,v 1.10 2008-10-06 03:22:33 blanqui Exp $ *)
+(* $Id: AContext.v,v 1.11 2008-10-08 08:27:51 blanqui Exp $ *)
 
 Set Implicit Arguments.
 
@@ -22,9 +22,7 @@ Variable Sig : Signature.
 
 Require Export ATerm.
 
-Notation term := (term Sig).
-Notation terms := (vector term).
-Notation "'args' f" := (terms (arity f)) (at level 70).
+Notation term := (term Sig). Notation terms := (vector term).
 
 (***********************************************************************)
 (** contexts and replacement of the hole *)
@@ -83,7 +81,7 @@ assert (C = Hole /\ u = Var x).
 apply var_eq_fill. exact H. destruct H0. exact H1.
 Qed.
 
-Lemma subterm_fun_elim : forall u f (ts : args f),
+Lemma subterm_fun_elim : forall u f ts,
   subterm u (Fun f ts) -> exists t, Vin t ts /\ subterm_eq u t.
 
 Proof.
@@ -93,7 +91,7 @@ clear H. simpl in H0. Funeqtac. subst ts. exists (fill C u). split.
 apply Vin_cast_intro. apply Vin_app_cons. unfold subterm_eq. exists C. refl.
 Qed.
 
-Lemma subterm_fun : forall f (ts : args f) u, Vin u ts -> subterm u (Fun f ts).
+Lemma subterm_fun : forall f ts u, Vin u ts -> subterm u (Fun f ts).
 
 Proof.
 intros. unfold subterm.
